v0.1 7/n: allocate_slab WIP

src/Slabs.fst
@@ -604,6 +604,37 @@ let s_vprop'
       (SeqUtils.init_u32_refined (U32.v md_count)))
 
 #push-options "--z3rlimit 75"
+assume val allocate_slab_aux_1_partial
+  (size_class: sc)
+  (slab_region: array U8.t{A.length slab_region = U32.v metadata_max * U32.v page_size})
+  (md_bm_region: array U64.t{A.length md_bm_region = U32.v metadata_max * 4})
+  (md_region: array (AL.cell status){A.length md_region = U32.v metadata_max})
+  (md_count: U32.t{0 < U32.v md_count /\ U32.v md_count < U32.v metadata_max})
+  (md_region_lv: G.erased (Seq.lseq status (U32.v md_count)))
+  (idx1: US.t{US.v idx1 < U32.v md_count})
+  (idx2 idx3: US.t)
+  (r1 r2 r3: ref US.t)
+  //: Steel (array U8.t)
+  : SteelT unit
+  (
+    vptr r1 `star`
+    vptr r2 `star`
+    vptr r3 `star`
+    (AL.varraylist pred1 pred2 pred3
+      (A.split_l md_region (u32_to_sz md_count))
+      (US.v idx1) (US.v idx2) (US.v idx3)) `star`
+    starseq
+      #(pos:U32.t{U32.v pos < U32.v md_count})
+      #(t size_class)
+      (f size_class slab_region md_bm_region md_count (Seq.upd (G.reveal md_region_lv) (US.v idx1) 1ul))
+      (f_lemma size_class slab_region md_bm_region md_count (Seq.upd (G.reveal md_region_lv) (US.v idx1) 1ul))
+      (SeqUtils.init_u32_refined (U32.v md_count))
+  )
+  (fun idxs ->
+    s_vprop' size_class slab_region md_bm_region md_count md_region r1 r2 r3
+  )
+
+
 assume val allocate_slab_aux_1_full
   (size_class: sc)
   (slab_region: array U8.t{A.length slab_region = U32.v metadata_max * U32.v page_size})
@@ -641,106 +672,6 @@ assume val allocate_slab_aux_1_full
   //  (A.split_l md_region (u32_to_sz md_count))
   //  (US.v idx1') (US.v idx2) (US.v idx3) idx1 in
   //write_in_place
-
-
-
-let a = 42
-
-//#push-options "--compat_pre_typed_indexed_effects"
-//#push-options "--z3rlimit 30"
-//let allocate_slab_aux_1_partial
-//  (size_class: sc)
-//  (partial_slabs_ptr empty_slabs_ptr: ref SL.t)
-//  (partial_slabs empty_slabs: SL.t)
-//  (cell_ptr: SL.t)
-//  (cell_content: SL.cell)
-//  (b: SL.blob)
-//  : Steel unit
-//  (
-//    slab_vprop size_class (snd b) (fst b) `star`
-//    (SAR.vptr cell_ptr `star`
-//    vptr empty_slabs_ptr `star`
-//    SL.llist (p_empty size_class) (SL.get_next cell_content) `star`
-//    vptr partial_slabs_ptr `star`
-//    SL.llist (p_partial size_class) partial_slabs)
-//  )
-//  (fun r ->
-//    SL.ind_llist (p_empty size_class) empty_slabs_ptr `star`
-//    SL.ind_llist (p_partial size_class) partial_slabs_ptr
-//  )
-//  (requires fun h0 ->
-//    let slab_vprop_data
-//      : t_of (slab_vprop size_class (snd b) (fst b))
-//      = h0 (slab_vprop size_class (snd b) (fst b)) in
-//    let md_seq : Seq.lseq U64.t 4 = dfst (fst slab_vprop_data) in
-//    sel partial_slabs_ptr h0 == partial_slabs /\
-//    SAR.sel cell_ptr h0 == cell_content /\
-//    is_partial size_class md_seq /\
-//    SL.get_data cell_content == b)
-//  (ensures fun h0 _ h1 ->
-//    True
-//  )
-//  =
-//  p_partial_pack size_class b (SL.get_data cell_content);
-//  let n_partial = SL.mk_cell partial_slabs (SL.get_data cell_content) in
-//  SAR.write cell_ptr n_partial;
-//  SL.pack_list (p_partial size_class)
-//    cell_ptr
-//    partial_slabs
-//    (SL.get_data cell_content);
-//  write partial_slabs_ptr cell_ptr;
-//  SL.pack_ind (p_partial size_class) partial_slabs_ptr cell_ptr;
-//  write empty_slabs_ptr (SL.get_next cell_content);
-//  SL.pack_ind (p_empty size_class)
-//    empty_slabs_ptr
-//    (SL.get_next cell_content)
-//
-//let allocate_slab_aux_1_full
-//  (size_class: sc)
-//  (full_slabs_ptr empty_slabs_ptr: ref SL.t)
-//  (full_slabs empty_slabs: SL.t)
-//  (cell_ptr: SL.t)
-//  (cell_content: SL.cell)
-//  (b: SL.blob)
-//  : Steel unit
-//  (
-//    slab_vprop size_class (snd b) (fst b) `star`
-//    (SAR.vptr cell_ptr `star`
-//    vptr empty_slabs_ptr `star`
-//    SL.llist (p_empty size_class) (SL.get_next cell_content) `star`
-//    vptr full_slabs_ptr `star`
-//    SL.llist (p_full size_class) full_slabs)
-//  )
-//  (fun r ->
-//    SL.ind_llist (p_empty size_class) empty_slabs_ptr `star`
-//    SL.ind_llist (p_full size_class) full_slabs_ptr
-//  )
-//  (requires fun h0 ->
-//    let slab_vprop_data
-//      : t_of (slab_vprop size_class (snd b) (fst b))
-//      = h0 (slab_vprop size_class (snd b) (fst b)) in
-//    let md_seq : Seq.lseq U64.t 4 = dfst (fst slab_vprop_data) in
-//    sel full_slabs_ptr h0 == full_slabs /\
-//    SAR.sel cell_ptr h0 == cell_content /\
-//    is_full size_class md_seq /\
-//    SL.get_data cell_content == b)
-//  (ensures fun h0 _ h1 ->
-//    True
-//  )
-//  =
-//  p_full_pack size_class b (SL.get_data cell_content);
-//  let n_full = SL.mk_cell full_slabs (SL.get_data cell_content) in
-//  SAR.write cell_ptr n_full;
-//  SL.pack_list (p_full size_class)
-//    cell_ptr
-//    full_slabs
-//    (SL.get_data cell_content);
-//  write full_slabs_ptr cell_ptr;
-//  SL.pack_ind (p_full size_class) full_slabs_ptr cell_ptr;
-//  write empty_slabs_ptr (SL.get_next cell_content);
-//  SL.pack_ind (p_empty size_class)
-//    empty_slabs_ptr
-//    (SL.get_next cell_content)
 
 //#push-options "--z3rlimit 50"
 //let allocate_slab_aux_1
@@ -788,6 +719,8 @@ let a = 42
 //  in
 //  let idx1 = read r1 in
 //  //let v1 = AL.read_in_place
+
+let _ = 42
 
 #push-options "--print_implicits"
 
@@ -896,54 +829,74 @@ let allocate_slab_aux_1
       r1 r2 r3;
     return r
   ) else (
-    sladmit ();
+    change_slprop_rel
+      (slab_vprop size_class
+        (slab_array slab_region (U32.uint_to_t (US.v idx1')))
+        (md_bm_array md_bm_region (U32.uint_to_t (US.v idx1'))))
+      (f size_class slab_region md_bm_region md_count
+        (Seq.upd md_region_lv (US.v idx1') 1ul)
+        (Seq.index (SeqUtils.init_u32_refined (U32.v md_count)) (US.v idx1')))
+      (fun x y -> x == y)
+      (fun _ -> admit ());
+    admit ();
+    starseq_upd_pack
+      #_
+      #(pos:U32.t{U32.v pos < U32.v md_count})
+      #(t size_class)
+      (f size_class slab_region md_bm_region md_count md_region_lv)
+      (f size_class slab_region md_bm_region md_count (Seq.upd (G.reveal md_region_lv) (US.v idx1') 1ul))
+      (f_lemma size_class slab_region md_bm_region md_count md_region_lv)
+      (f_lemma size_class slab_region md_bm_region md_count (Seq.upd (G.reveal md_region_lv) (US.v idx1') 1ul))
+      (SeqUtils.init_u32_refined (U32.v md_count))
+      (SeqUtils.init_u32_refined (U32.v md_count))
+      (US.v idx1');
+    allocate_slab_aux_1_partial
+      size_class
+      slab_region
+      md_bm_region
+      md_region
+      md_count
+      md_region_lv
+      idx1' idx2 idx3
+      r1 r2 r3;
     return r
   )
 
-//inline_for_extraction noextract
-//let allocate_slab_aux_2
-//  (sc: sc)
-//  (partial_slabs_ptr empty_slabs_ptr: ref SL.t)
-//  (partial_slabs empty_slabs: SL.t)
-//  : Steel (array U8.t)
-//  (
-//  vptr empty_slabs_ptr `star`
-//  SL.llist (p_empty sc) empty_slabs `star`
-//  vptr partial_slabs_ptr `star`
-//  SL.llist (p_partial sc) partial_slabs)
-//  (fun r ->
-//  A.varray r `star`
-//  SL.ind_llist (p_empty sc) empty_slabs_ptr `star`
-//  SL.ind_llist (p_partial sc) partial_slabs_ptr)
-//  (requires fun h0 ->
-//    sel partial_slabs_ptr h0 == partial_slabs /\
-//    sel empty_slabs_ptr h0 == empty_slabs /\
-//    not (SL.is_null_t partial_slabs))
-//  (ensures fun _ _ _ -> True)
-//  =
-//  let n_partial = SL.unpack_list (p_partial sc) partial_slabs in
-//  let b = SL.get_data n_partial in
-//  p_partial_unpack sc
-//    (SL.get_data n_partial)
-//    b;
-//  let r = allocate_slot sc (fst b) (snd b) in
-//  let blob0
-//    : G.erased (t_of (slab_vprop sc (snd b) (fst b)))
-//    = gget (slab_vprop sc (snd b) (fst b)) in
-//  let v0 : G.erased (Seq.lseq U64.t 4) = dfst (fst blob0) in
-//  // TODO: false, but ok for now as nb_slots size_class > 1
-//  assume (is_partial sc v0);
-//  p_partial_pack sc
-//    b
-//    (SL.get_data n_partial);
-//  SL.pack_list (p_partial sc)
-//    partial_slabs
-//    (SL.get_next n_partial)
-//    (SL.get_data n_partial);
-//  SL.pack_ind (p_partial sc) partial_slabs_ptr partial_slabs;
-//  SL.pack_ind (p_empty sc) empty_slabs_ptr empty_slabs;
-//  return r
-//#pop-options
+assume val allocate_slab_aux_2
+  (size_class: sc)
+  (slab_region: array U8.t{A.length slab_region = U32.v metadata_max * U32.v page_size})
+  (md_bm_region: array U64.t{A.length md_bm_region = U32.v metadata_max * 4})
+  (md_region: array (AL.cell status){A.length md_region = U32.v metadata_max})
+  (md_count: U32.t{0 < U32.v md_count /\ U32.v md_count < U32.v metadata_max})
+  (md_region_lv: G.erased (Seq.lseq status (U32.v md_count)))
+  (idx1 idx2 idx3: US.t)
+  (r1 r2 r3: ref US.t)
+  : Steel (array U8.t)
+  (
+    vptr r1 `star`
+    vptr r2 `star`
+    vptr r3 `star`
+    (AL.varraylist pred1 pred2 pred3
+      (A.split_l md_region (u32_to_sz md_count))
+      (US.v idx1) (US.v idx2) (US.v idx3)) `star`
+    starseq
+      #(pos:U32.t{U32.v pos < U32.v md_count})
+      #(t size_class)
+      (f size_class slab_region md_bm_region md_count md_region_lv)
+      (f_lemma size_class slab_region md_bm_region md_count md_region_lv)
+      (SeqUtils.init_u32_refined (U32.v md_count))
+  )
+  (fun r ->
+    A.varray r `star`
+    s_vprop' size_class slab_region md_bm_region md_count md_region r1 r2 r3
+  )
+  (requires fun h0 ->
+    sel r1 h0 == idx1 /\
+    sel r2 h0 == idx2 /\
+    sel r3 h0 == idx3 /\
+    idx2 <> AL.null_ptr
+  )
+  (ensures fun _ _ _ -> True)
 
 #push-options "--z3rlimit 30"
 let alloc_metadata_aux
@@ -1023,46 +976,47 @@ let empty_md_is_properly_zeroed
   zf_b_slice (Seq.slice bm 0 64) 0 (64 - U32.v bound2)
 #pop-options
 
-#push-options "--z3rlimit 100 --compat_pre_typed_indexed_effects"
-let alloc_metadata_aux2
-  (md_count: U32.t{U32.v md_count < U32.v metadata_max})
-  (size_class: sc)
-  (slab_region: array U8.t{A.length slab_region = U32.v metadata_max * U32.v page_size})
-  (md_bm_region: array U64.t{A.length md_bm_region = U32.v metadata_max * 4})
-  (md_region: array SL.cell{A.length md_region = U32.v metadata_max})
-  : Steel (SL.t & (G.erased U32.t))
-  (
-    A.varray (A.split_r slab_region (u32_to_sz (U32.mul md_count page_size))) `star`
-    A.varray (A.split_r md_bm_region (u32_to_sz (U32.mul md_count 4ul))) `star`
-    A.varray (A.split_r md_region (u32_to_sz md_count))
-  )
-  (fun r ->
-    SL.llist (p_empty size_class) (fst r) `star`
-    A.varray (A.split_r slab_region (u32_to_sz (U32.mul (U32.add md_count 1ul) page_size))) `star`
-    A.varray (A.split_r md_bm_region (u32_to_sz (U32.mul (U32.add md_count 1ul) 4ul))) `star`
-    A.varray (A.split_r md_region (u32_to_sz (U32.add md_count 1ul)))
-  )
-  (requires fun h0 ->
-    (U32.v page_size) % (U32.v size_class) == 0 /\
-    zf_u8 (A.asel (A.split_r slab_region (u32_to_sz (U32.mul md_count page_size))) h0) /\
-    zf_u64 (A.asel (A.split_r md_bm_region (u32_to_sz (U32.mul md_count 4ul))) h0))
-  (ensures fun h0 r h1 ->
-    L.length (SL.v_llist (p_empty size_class) (fst r) h1) = 1 /\
-    G.reveal (snd r) = U32.add md_count 1ul /\
-    U32.v (G.reveal (snd r)) <= U32.v metadata_max /\
-    zf_u8 (A.asel (A.split_r slab_region (u32_to_sz (U32.mul (U32.add md_count 1ul) page_size))) h1) /\
-    zf_u64 (A.asel (A.split_r md_bm_region (u32_to_sz (U32.mul (U32.add md_count 1ul) 4ul))) h1)
-  )
-  =
-  let b : SL.blob = alloc_metadata_aux md_count size_class slab_region md_bm_region md_region in
-  empty_md_is_properly_zeroed size_class;
-  intro_slab_vprop size_class (fst b) (Seq.create 4 0UL) (snd b);
-  zeroes_impl_empty size_class (Seq.create 4 0UL);
-  p_empty_pack size_class b b;
-  SAR.intro_vptr (md_array md_region md_count);
-  SL.intro_singleton_llist_no_alloc (p_empty size_class) (md_array md_region md_count) b;
-  return (md_array md_region md_count, G.hide (U32.add md_count 1ul))
-#pop-options
+//TODO: remove
+//#push-options "--z3rlimit 100 --compat_pre_typed_indexed_effects"
+//let alloc_metadata_aux2
+//  (md_count: U32.t{U32.v md_count < U32.v metadata_max})
+//  (size_class: sc)
+//  (slab_region: array U8.t{A.length slab_region = U32.v metadata_max * U32.v page_size})
+//  (md_bm_region: array U64.t{A.length md_bm_region = U32.v metadata_max * 4})
+//  (md_region: array SL.cell{A.length md_region = U32.v metadata_max})
+//  : Steel (SL.t & (G.erased U32.t))
+//  (
+//    A.varray (A.split_r slab_region (u32_to_sz (U32.mul md_count page_size))) `star`
+//    A.varray (A.split_r md_bm_region (u32_to_sz (U32.mul md_count 4ul))) `star`
+//    A.varray (A.split_r md_region (u32_to_sz md_count))
+//  )
+//  (fun r ->
+//    SL.llist (p_empty size_class) (fst r) `star`
+//    A.varray (A.split_r slab_region (u32_to_sz (U32.mul (U32.add md_count 1ul) page_size))) `star`
+//    A.varray (A.split_r md_bm_region (u32_to_sz (U32.mul (U32.add md_count 1ul) 4ul))) `star`
+//    A.varray (A.split_r md_region (u32_to_sz (U32.add md_count 1ul)))
+//  )
+//  (requires fun h0 ->
+//    (U32.v page_size) % (U32.v size_class) == 0 /\
+//    zf_u8 (A.asel (A.split_r slab_region (u32_to_sz (U32.mul md_count page_size))) h0) /\
+//    zf_u64 (A.asel (A.split_r md_bm_region (u32_to_sz (U32.mul md_count 4ul))) h0))
+//  (ensures fun h0 r h1 ->
+//    L.length (SL.v_llist (p_empty size_class) (fst r) h1) = 1 /\
+//    G.reveal (snd r) = U32.add md_count 1ul /\
+//    U32.v (G.reveal (snd r)) <= U32.v metadata_max /\
+//    zf_u8 (A.asel (A.split_r slab_region (u32_to_sz (U32.mul (U32.add md_count 1ul) page_size))) h1) /\
+//    zf_u64 (A.asel (A.split_r md_bm_region (u32_to_sz (U32.mul (U32.add md_count 1ul) 4ul))) h1)
+//  )
+//  =
+//  let b : SL.blob = alloc_metadata_aux md_count size_class slab_region md_bm_region md_region in
+//  empty_md_is_properly_zeroed size_class;
+//  intro_slab_vprop size_class (fst b) (Seq.create 4 0UL) (snd b);
+//  zeroes_impl_empty size_class (Seq.create 4 0UL);
+//  p_empty_pack size_class b b;
+//  SAR.intro_vptr (md_array md_region md_count);
+//  SL.intro_singleton_llist_no_alloc (p_empty size_class) (md_array md_region md_count) b;
+//  return (md_array md_region md_count, G.hide (U32.add md_count 1ul))
+//#pop-options
 
 let alloc_metadata_sl1
   (slab_region: array U8.t{A.length slab_region = U32.v metadata_max * U32.v page_size})
@@ -1138,141 +1092,143 @@ let alloc_metadata_sl2
   =
   ()
 
-#push-options "--z3rlimit 100"
-let alloc_metadata
-  (size_class: sc)
-  (slab_region: array U8.t{A.length slab_region = U32.v metadata_max * U32.v page_size})
-  (md_bm_region: array U64.t{A.length md_bm_region = U32.v metadata_max * 4})
-  (md_region: array SL.cell{A.length md_region = U32.v metadata_max})
-  (md_count: ref U32.t)
-  (md_count_v: G.erased (v:U32.t{U32.v v < U32.v metadata_max}))
-  : Steel (SL.t & G.erased U32.t)
-  (
-    vptr md_count `star`
-    A.varray (A.split_r slab_region (u32_to_sz (U32.mul (G.reveal md_count_v) page_size))) `star`
-    A.varray (A.split_r md_bm_region (u32_to_sz (U32.mul (G.reveal md_count_v) 4ul))) `star`
-    A.varray (A.split_r md_region (u32_to_sz (G.reveal md_count_v)))
-  )
-  (fun r ->
-    vptr md_count `star`
-    SL.llist (p_empty size_class) (fst r) `star`
-    A.varray (A.split_r slab_region (u32_to_sz (U32.mul (U32.add (G.reveal md_count_v) 1ul) page_size))) `star`
-    A.varray (A.split_r md_bm_region (u32_to_sz (U32.mul (U32.add (G.reveal md_count_v) 1ul) 4ul))) `star`
-    A.varray (A.split_r md_region (u32_to_sz (U32.add (G.reveal md_count_v) 1ul)))
-  )
-  (requires fun h0 ->
-    (U32.v page_size) % (U32.v size_class) == 0 /\
-    zf_u8 (A.asel (A.split_r slab_region (u32_to_sz (U32.mul (G.reveal md_count_v) page_size))) h0) /\
-    zf_u64 (A.asel (A.split_r md_bm_region (u32_to_sz (U32.mul (G.reveal md_count_v) 4ul))) h0) /\
-    sel md_count h0 = G.reveal md_count_v
-  )
-  (ensures fun h0 r h1 ->
-    L.length (SL.v_llist (p_empty size_class) (fst r) h1) = 1 /\
-    sel md_count h0 = G.reveal md_count_v /\
-    sel md_count h1 = U32.add (sel md_count h0) 1ul /\
-    sel md_count h1 = G.reveal (snd r) /\
-    zf_u8 (A.asel (A.split_r slab_region (u32_to_sz (U32.mul (U32.add (G.reveal md_count_v) 1ul) page_size))) h1) /\
-    zf_u64 (A.asel (A.split_r md_bm_region (u32_to_sz (U32.mul (U32.add (G.reveal md_count_v) 1ul) 4ul))) h1)
-  )
-  =
-  let md_count_v0 = read md_count in
-  assert (md_count_v0 == G.reveal md_count_v);
-  change_equal_slprop
-    (A.varray (A.split_r slab_region (u32_to_sz (U32.mul (G.reveal md_count_v) page_size))) `star`
-    A.varray (A.split_r md_bm_region (u32_to_sz (U32.mul (G.reveal md_count_v) 4ul))) `star`
-    A.varray (A.split_r md_region (u32_to_sz (G.reveal md_count_v))))
-    (A.varray (A.split_r slab_region (u32_to_sz (U32.mul md_count_v0 page_size))) `star`
-    A.varray (A.split_r md_bm_region (u32_to_sz (U32.mul md_count_v0 4ul))) `star`
-    A.varray (A.split_r md_region (u32_to_sz md_count_v0)));
-  let r = alloc_metadata_aux2 md_count_v0 size_class slab_region md_bm_region md_region in
-  assert (U32.add md_count_v0 1ul == U32.add (G.reveal md_count_v) 1ul);
-  change_equal_slprop
-    (A.varray (A.split_r slab_region (u32_to_sz (U32.mul (U32.add md_count_v0 1ul) page_size))) `star`
-    A.varray (A.split_r md_bm_region (u32_to_sz (U32.mul (U32.add md_count_v0 1ul) 4ul))) `star`
-    A.varray (A.split_r md_region (u32_to_sz (U32.add md_count_v0 1ul))))
-    (A.varray (A.split_r slab_region (u32_to_sz (U32.mul (U32.add (G.reveal md_count_v) 1ul) page_size))) `star`
-    A.varray (A.split_r md_bm_region (u32_to_sz (U32.mul (U32.add (G.reveal md_count_v) 1ul) 4ul))) `star`
-    A.varray (A.split_r md_region (u32_to_sz (U32.add (G.reveal md_count_v) 1ul))));
-  write md_count (U32.add md_count_v0 1ul);
-  let md_count_v1 = read md_count in
-  assert (md_count_v1 == G.reveal (snd r));
-  //assert (U32.v md_count_v1 <= U32.v metadata_max);
-  return r
-#pop-options
+////TODO: remove
+//#push-options "--z3rlimit 100"
+//let alloc_metadata
+//  (size_class: sc)
+//  (slab_region: array U8.t{A.length slab_region = U32.v metadata_max * U32.v page_size})
+//  (md_bm_region: array U64.t{A.length md_bm_region = U32.v metadata_max * 4})
+//  (md_region: array SL.cell{A.length md_region = U32.v metadata_max})
+//  (md_count: ref U32.t)
+//  (md_count_v: G.erased (v:U32.t{U32.v v < U32.v metadata_max}))
+//  : Steel (SL.t & G.erased U32.t)
+//  (
+//    vptr md_count `star`
+//    A.varray (A.split_r slab_region (u32_to_sz (U32.mul (G.reveal md_count_v) page_size))) `star`
+//    A.varray (A.split_r md_bm_region (u32_to_sz (U32.mul (G.reveal md_count_v) 4ul))) `star`
+//    A.varray (A.split_r md_region (u32_to_sz (G.reveal md_count_v)))
+//  )
+//  (fun r ->
+//    vptr md_count `star`
+//    SL.llist (p_empty size_class) (fst r) `star`
+//    A.varray (A.split_r slab_region (u32_to_sz (U32.mul (U32.add (G.reveal md_count_v) 1ul) page_size))) `star`
+//    A.varray (A.split_r md_bm_region (u32_to_sz (U32.mul (U32.add (G.reveal md_count_v) 1ul) 4ul))) `star`
+//    A.varray (A.split_r md_region (u32_to_sz (U32.add (G.reveal md_count_v) 1ul)))
+//  )
+//  (requires fun h0 ->
+//    (U32.v page_size) % (U32.v size_class) == 0 /\
+//    zf_u8 (A.asel (A.split_r slab_region (u32_to_sz (U32.mul (G.reveal md_count_v) page_size))) h0) /\
+//    zf_u64 (A.asel (A.split_r md_bm_region (u32_to_sz (U32.mul (G.reveal md_count_v) 4ul))) h0) /\
+//    sel md_count h0 = G.reveal md_count_v
+//  )
+//  (ensures fun h0 r h1 ->
+//    L.length (SL.v_llist (p_empty size_class) (fst r) h1) = 1 /\
+//    sel md_count h0 = G.reveal md_count_v /\
+//    sel md_count h1 = U32.add (sel md_count h0) 1ul /\
+//    sel md_count h1 = G.reveal (snd r) /\
+//    zf_u8 (A.asel (A.split_r slab_region (u32_to_sz (U32.mul (U32.add (G.reveal md_count_v) 1ul) page_size))) h1) /\
+//    zf_u64 (A.asel (A.split_r md_bm_region (u32_to_sz (U32.mul (U32.add (G.reveal md_count_v) 1ul) 4ul))) h1)
+//  )
+//  =
+//  let md_count_v0 = read md_count in
+//  assert (md_count_v0 == G.reveal md_count_v);
+//  change_equal_slprop
+//    (A.varray (A.split_r slab_region (u32_to_sz (U32.mul (G.reveal md_count_v) page_size))) `star`
+//    A.varray (A.split_r md_bm_region (u32_to_sz (U32.mul (G.reveal md_count_v) 4ul))) `star`
+//    A.varray (A.split_r md_region (u32_to_sz (G.reveal md_count_v))))
+//    (A.varray (A.split_r slab_region (u32_to_sz (U32.mul md_count_v0 page_size))) `star`
+//    A.varray (A.split_r md_bm_region (u32_to_sz (U32.mul md_count_v0 4ul))) `star`
+//    A.varray (A.split_r md_region (u32_to_sz md_count_v0)));
+//  let r = alloc_metadata_aux2 md_count_v0 size_class slab_region md_bm_region md_region in
+//  assert (U32.add md_count_v0 1ul == U32.add (G.reveal md_count_v) 1ul);
+//  change_equal_slprop
+//    (A.varray (A.split_r slab_region (u32_to_sz (U32.mul (U32.add md_count_v0 1ul) page_size))) `star`
+//    A.varray (A.split_r md_bm_region (u32_to_sz (U32.mul (U32.add md_count_v0 1ul) 4ul))) `star`
+//    A.varray (A.split_r md_region (u32_to_sz (U32.add md_count_v0 1ul))))
+//    (A.varray (A.split_r slab_region (u32_to_sz (U32.mul (U32.add (G.reveal md_count_v) 1ul) page_size))) `star`
+//    A.varray (A.split_r md_bm_region (u32_to_sz (U32.mul (U32.add (G.reveal md_count_v) 1ul) 4ul))) `star`
+//    A.varray (A.split_r md_region (u32_to_sz (U32.add (G.reveal md_count_v) 1ul))));
+//  write md_count (U32.add md_count_v0 1ul);
+//  let md_count_v1 = read md_count in
+//  assert (md_count_v1 == G.reveal (snd r));
+//  //assert (U32.v md_count_v1 <= U32.v metadata_max);
+//  return r
+//#pop-options
 
-//TODO: move it inside SL lib
-let unpack_list_singleton
-  (p: SL.blob -> vprop)
-  (ptr: SL.t)
-  : Steel SL.cell
-  (SL.llist p ptr)
-  (fun n -> SAR.vptr ptr `star` p (SL.get_data n))
-  (requires fun h0 ->
-    L.length (SL.v_llist p ptr h0) = 1)
-  (ensures fun h0 n h1 ->
-    SL.v_llist p ptr h0 ==
-      (SL.get_data (SAR.sel ptr h1)) :: [] /\
-    SAR.sel ptr h1 == n)
-  =
-  SL.cons_is_not_null p ptr;
-  let n = SL.unpack_list p ptr in
-  //TODO: FIXME (add AVL-like helper)
-  drop (SL.llist p (SL.get_next n));
-  return n
+////TODO: move it inside SL lib
+//let unpack_list_singleton
+//  (p: SL.blob -> vprop)
+//  (ptr: SL.t)
+//  : Steel SL.cell
+//  (SL.llist p ptr)
+//  (fun n -> SAR.vptr ptr `star` p (SL.get_data n))
+//  (requires fun h0 ->
+//    L.length (SL.v_llist p ptr h0) = 1)
+//  (ensures fun h0 n h1 ->
+//    SL.v_llist p ptr h0 ==
+//      (SL.get_data (SAR.sel ptr h1)) :: [] /\
+//    SAR.sel ptr h1 == n)
+//  =
+//  SL.cons_is_not_null p ptr;
+//  let n = SL.unpack_list p ptr in
+//  //TODO: FIXME (add AVL-like helper)
+//  drop (SL.llist p (SL.get_next n));
+//  return n
 
-#push-options "--z3rlimit 100"
-let alloc_metadata'
-  (size_class: sc)
-  (slab_region: array U8.t{A.length slab_region = U32.v metadata_max * U32.v page_size})
-  (md_bm_region: array U64.t{A.length md_bm_region = U32.v metadata_max * 4})
-  (md_region: array SL.cell{A.length md_region = U32.v metadata_max})
-  (md_count: ref U32.t)
-  (md_count_v: G.erased (v:U32.t{U32.v v < U32.v metadata_max}))
-  : Steel SL.t
-  (
-    vptr md_count `star`
-    (A.varray (A.split_r slab_region (u32_to_sz (U32.mul (G.reveal md_count_v) page_size)))
-      `vrefine` zf_u8) `star`
-    (A.varray (A.split_r md_bm_region (u32_to_sz (U32.mul (G.reveal md_count_v) 4ul)))
-      `vrefine` zf_u64) `star`
-    A.varray (A.split_r md_region (u32_to_sz (G.reveal md_count_v)))
-  )
-  (fun r ->
-    vptr md_count `star`
-    SL.llist (p_empty size_class) r `star`
-    (A.varray (A.split_r slab_region (u32_to_sz (U32.mul (U32.add (G.reveal md_count_v) 1ul) page_size)))
-      `vrefine` zf_u8) `star`
-    (A.varray (A.split_r md_bm_region (u32_to_sz (U32.mul (U32.add (G.reveal md_count_v) 1ul) 4ul)))
-      `vrefine` zf_u64) `star`
-    A.varray (A.split_r md_region (u32_to_sz (U32.add (G.reveal md_count_v) 1ul)))
-  )
-  (requires fun h0 ->
-    sel md_count h0 = G.reveal md_count_v /\
-    (U32.v page_size) % (U32.v size_class) == 0
-  )
-  (ensures fun h0 r h1 ->
-    L.length (SL.v_llist (p_empty size_class) r h1) = 1 /\
-    sel md_count h0 = G.reveal md_count_v /\
-    sel md_count h1 = U32.add (sel md_count h0) 1ul /\
-    U32.v (U32.add (sel md_count h0) 1ul) <= U32.v metadata_max
-    //sel md_count h1 = G.reveal (snd r)
-  )
-  =
-  elim_vrefine
-    (A.varray (A.split_r slab_region (u32_to_sz (U32.mul (G.reveal md_count_v) page_size))))
-    zf_u8;
-  elim_vrefine
-    (A.varray (A.split_r md_bm_region (u32_to_sz (U32.mul (G.reveal md_count_v) 4ul))))
-    zf_u64;
-  let r = alloc_metadata size_class slab_region md_bm_region md_region md_count md_count_v in
-  intro_vrefine
-    (A.varray (A.split_r slab_region (u32_to_sz (U32.mul (U32.add (G.reveal md_count_v) 1ul) page_size))))
-    zf_u8;
-  intro_vrefine
-    (A.varray (A.split_r md_bm_region (u32_to_sz (U32.mul (U32.add (G.reveal md_count_v) 1ul) 4ul))))
-    zf_u64;
-  return (fst r)
-#pop-options
+//TODO: remove
+//#push-options "--z3rlimit 100"
+//let alloc_metadata'
+//  (size_class: sc)
+//  (slab_region: array U8.t{A.length slab_region = U32.v metadata_max * U32.v page_size})
+//  (md_bm_region: array U64.t{A.length md_bm_region = U32.v metadata_max * 4})
+//  (md_region: array SL.cell{A.length md_region = U32.v metadata_max})
+//  (md_count: ref U32.t)
+//  (md_count_v: G.erased (v:U32.t{U32.v v < U32.v metadata_max}))
+//  : Steel SL.t
+//  (
+//    vptr md_count `star`
+//    (A.varray (A.split_r slab_region (u32_to_sz (U32.mul (G.reveal md_count_v) page_size)))
+//      `vrefine` zf_u8) `star`
+//    (A.varray (A.split_r md_bm_region (u32_to_sz (U32.mul (G.reveal md_count_v) 4ul)))
+//      `vrefine` zf_u64) `star`
+//    A.varray (A.split_r md_region (u32_to_sz (G.reveal md_count_v)))
+//  )
+//  (fun r ->
+//    vptr md_count `star`
+//    SL.llist (p_empty size_class) r `star`
+//    (A.varray (A.split_r slab_region (u32_to_sz (U32.mul (U32.add (G.reveal md_count_v) 1ul) page_size)))
+//      `vrefine` zf_u8) `star`
+//    (A.varray (A.split_r md_bm_region (u32_to_sz (U32.mul (U32.add (G.reveal md_count_v) 1ul) 4ul)))
+//      `vrefine` zf_u64) `star`
+//    A.varray (A.split_r md_region (u32_to_sz (U32.add (G.reveal md_count_v) 1ul)))
+//  )
+//  (requires fun h0 ->
+//    sel md_count h0 = G.reveal md_count_v /\
+//    (U32.v page_size) % (U32.v size_class) == 0
+//  )
+//  (ensures fun h0 r h1 ->
+//    L.length (SL.v_llist (p_empty size_class) r h1) = 1 /\
+//    sel md_count h0 = G.reveal md_count_v /\
+//    sel md_count h1 = U32.add (sel md_count h0) 1ul /\
+//    U32.v (U32.add (sel md_count h0) 1ul) <= U32.v metadata_max
+//    //sel md_count h1 = G.reveal (snd r)
+//  )
+//  =
+//  elim_vrefine
+//    (A.varray (A.split_r slab_region (u32_to_sz (U32.mul (G.reveal md_count_v) page_size))))
+//    zf_u8;
+//  elim_vrefine
+//    (A.varray (A.split_r md_bm_region (u32_to_sz (U32.mul (G.reveal md_count_v) 4ul))))
+//    zf_u64;
+//  let r = alloc_metadata size_class slab_region md_bm_region md_region md_count md_count_v in
+//  intro_vrefine
+//    (A.varray (A.split_r slab_region (u32_to_sz (U32.mul (U32.add (G.reveal md_count_v) 1ul) page_size))))
+//    zf_u8;
+//  intro_vrefine
+//    (A.varray (A.split_r md_bm_region (u32_to_sz (U32.mul (U32.add (G.reveal md_count_v) 1ul) 4ul))))
+//    zf_u64;
+//  return (fst r)
+//#pop-options
 
 open SteelVRefineDep
 
@@ -1360,84 +1316,84 @@ let vp_aux_equal_lemma
   )
   = ()
 
-(*)
-#push-options "--compat_pre_typed_indexed_effects --z3rlimit 100"
-let alloc_metadata2
-  (size_class: sc)
-  (slab_region: array U8.t{A.length slab_region = U32.v metadata_max * U32.v page_size})
-  (md_bm_region: array U64.t{A.length md_bm_region = U32.v metadata_max * 4})
-  (md_region: array SL.cell{A.length md_region = U32.v metadata_max})
-  (md_count: ref U32.t)
-  : Steel SL.t
-  (
-    vrefinedep
-      (vptr md_count)
-      (fun x -> U32.v x <= U32.v metadata_max == true)
-      (fun v -> vp_aux slab_region md_bm_region md_region v)
-  )
-  (fun r ->
-    SL.llist (p_empty size_class) r `star`
-    vrefinedep
-      (vptr md_count)
-      (fun x -> U32.v x <= U32.v metadata_max == true)
-      (fun v -> vp_aux slab_region md_bm_region md_region v)
-  )
-  (requires fun h0 ->
-    let x = h0 (
-      vrefinedep
-        (vptr md_count)
-        (fun x -> U32.v x <= U32.v metadata_max == true)
-        (fun v -> vp_aux slab_region md_bm_region md_region v)
-      ) in
-    U32.v (dfst x) < U32.v metadata_max /\
-    (U32.v page_size) % (U32.v size_class) == 0)
-  (ensures fun h0 r h1 ->
-    FStar.List.Tot.length (SL.v_llist (p_empty size_class) r h1) = 1
-  )
-  =
-  let x
-    = elim_vrefinedep
-    (vptr md_count)
-    (fun x -> U32.v x <= U32.v metadata_max == true)
-    (fun v -> vp_aux slab_region md_bm_region md_region v)
-  in
-  let x'
-    : G.erased (x:U32.t{U32.v x < U32.v metadata_max})
-    = G.hide (G.reveal x <: x:U32.t{U32.v x < U32.v metadata_max}) in
-  //TODO: hideous coercion that leads to 2 change_slprop_rel
-  change_equal_slprop
-    (vp_aux slab_region md_bm_region md_region (G.reveal x))
-    (vp_aux_lt slab_region md_bm_region md_region (G.reveal x'));
-  change_slprop_rel
-    (vp_aux_lt slab_region md_bm_region md_region (G.reveal x'))
-    ((A.varray (A.split_r slab_region (u32_to_sz (U32.mul (G.reveal x') page_size)))
-      `vrefine` zf_u8) `star`
-    (A.varray (A.split_r md_bm_region (u32_to_sz (U32.mul (G.reveal x') 4ul)))
-      `vrefine` zf_u64) `star`
-    A.varray (A.split_r md_region (u32_to_sz (G.reveal x'))))
-    (fun x y -> x == y)
-    (fun m -> vp_aux_lt_equal_lemma slab_region md_bm_region md_region (G.reveal x') m);
-  let r = alloc_metadata' size_class slab_region md_bm_region md_region md_count x' in
-  //TODO: hideous coercion that leads to 2 change_slprop_rel
-  change_slprop_rel
-    ((A.varray (A.split_r slab_region (u32_to_sz (U32.mul (U32.add (G.reveal x') 1ul) page_size)))
-      `vrefine` zf_u8) `star`
-    (A.varray (A.split_r md_bm_region (u32_to_sz (U32.mul (U32.add (G.reveal x') 1ul) 4ul)))
-      `vrefine` zf_u64) `star`
-    A.varray (A.split_r md_region (u32_to_sz (U32.add (G.reveal x') 1ul))))
-    (vp_aux slab_region md_bm_region md_region (U32.add (G.reveal x') 1ul))
-    (fun x y -> x == y)
-    (fun m -> vp_aux_equal_lemma slab_region md_bm_region md_region (U32.add (G.reveal x') 1ul) m);
-  change_equal_slprop
-    (vp_aux slab_region md_bm_region md_region (U32.add (G.reveal x') 1ul))
-    (vp_aux slab_region md_bm_region md_region (U32.add (G.reveal x) 1ul));
-  intro_vrefinedep
-    (vptr md_count)
-    (fun x -> U32.v x <= U32.v metadata_max == true)
-    (fun v -> vp_aux slab_region md_bm_region md_region v)
-    (vp_aux slab_region md_bm_region md_region (U32.add (G.reveal x) 1ul));
-  return r
-#pop-options
+////TODO: remove
+//#push-options "--compat_pre_typed_indexed_effects --z3rlimit 100"
+//let alloc_metadata2
+//  (size_class: sc)
+//  (slab_region: array U8.t{A.length slab_region = U32.v metadata_max * U32.v page_size})
+//  (md_bm_region: array U64.t{A.length md_bm_region = U32.v metadata_max * 4})
+//  (md_region: array SL.cell{A.length md_region = U32.v metadata_max})
+//  (md_count: ref U32.t)
+//  : Steel SL.t
+//  (
+//    vrefinedep
+//      (vptr md_count)
+//      (fun x -> U32.v x <= U32.v metadata_max == true)
+//      (fun v -> vp_aux slab_region md_bm_region md_region v)
+//  )
+//  (fun r ->
+//    SL.llist (p_empty size_class) r `star`
+//    vrefinedep
+//      (vptr md_count)
+//      (fun x -> U32.v x <= U32.v metadata_max == true)
+//      (fun v -> vp_aux slab_region md_bm_region md_region v)
+//  )
+//  (requires fun h0 ->
+//    let x = h0 (
+//      vrefinedep
+//        (vptr md_count)
+//        (fun x -> U32.v x <= U32.v metadata_max == true)
+//        (fun v -> vp_aux slab_region md_bm_region md_region v)
+//      ) in
+//    U32.v (dfst x) < U32.v metadata_max /\
+//    (U32.v page_size) % (U32.v size_class) == 0)
+//  (ensures fun h0 r h1 ->
+//    FStar.List.Tot.length (SL.v_llist (p_empty size_class) r h1) = 1
+//  )
+//  =
+//  let x
+//    = elim_vrefinedep
+//    (vptr md_count)
+//    (fun x -> U32.v x <= U32.v metadata_max == true)
+//    (fun v -> vp_aux slab_region md_bm_region md_region v)
+//  in
+//  let x'
+//    : G.erased (x:U32.t{U32.v x < U32.v metadata_max})
+//    = G.hide (G.reveal x <: x:U32.t{U32.v x < U32.v metadata_max}) in
+//  //TODO: hideous coercion that leads to 2 change_slprop_rel
+//  change_equal_slprop
+//    (vp_aux slab_region md_bm_region md_region (G.reveal x))
+//    (vp_aux_lt slab_region md_bm_region md_region (G.reveal x'));
+//  change_slprop_rel
+//    (vp_aux_lt slab_region md_bm_region md_region (G.reveal x'))
+//    ((A.varray (A.split_r slab_region (u32_to_sz (U32.mul (G.reveal x') page_size)))
+//      `vrefine` zf_u8) `star`
+//    (A.varray (A.split_r md_bm_region (u32_to_sz (U32.mul (G.reveal x') 4ul)))
+//      `vrefine` zf_u64) `star`
+//    A.varray (A.split_r md_region (u32_to_sz (G.reveal x'))))
+//    (fun x y -> x == y)
+//    (fun m -> vp_aux_lt_equal_lemma slab_region md_bm_region md_region (G.reveal x') m);
+//  let r = alloc_metadata' size_class slab_region md_bm_region md_region md_count x' in
+//  //TODO: hideous coercion that leads to 2 change_slprop_rel
+//  change_slprop_rel
+//    ((A.varray (A.split_r slab_region (u32_to_sz (U32.mul (U32.add (G.reveal x') 1ul) page_size)))
+//      `vrefine` zf_u8) `star`
+//    (A.varray (A.split_r md_bm_region (u32_to_sz (U32.mul (U32.add (G.reveal x') 1ul) 4ul)))
+//      `vrefine` zf_u64) `star`
+//    A.varray (A.split_r md_region (u32_to_sz (U32.add (G.reveal x') 1ul))))
+//    (vp_aux slab_region md_bm_region md_region (U32.add (G.reveal x') 1ul))
+//    (fun x y -> x == y)
+//    (fun m -> vp_aux_equal_lemma slab_region md_bm_region md_region (U32.add (G.reveal x') 1ul) m);
+//  change_equal_slprop
+//    (vp_aux slab_region md_bm_region md_region (U32.add (G.reveal x') 1ul))
+//    (vp_aux slab_region md_bm_region md_region (U32.add (G.reveal x) 1ul));
+//  intro_vrefinedep
+//    (vptr md_count)
+//    (fun x -> U32.v x <= U32.v metadata_max == true)
+//    (fun v -> vp_aux slab_region md_bm_region md_region v)
+//    (vp_aux slab_region md_bm_region md_region (U32.add (G.reveal x) 1ul));
+//  return r
+//#pop-options
 
 #push-options "--compat_pre_typed_indexed_effects --z3rlimit 100"
 inline_for_extraction noextract
